Fix program logic bug

Examples/LockSpec.v
@@ -2,6 +2,9 @@ From LHL.Core Require Import
   Program
   Specs.
 
+From Coq Require Import
+  Program.Equality.
+
 Variant LockSig : ESig :=
 | Acq : LockSig unit
 | Rel : LockSig unit.
@@ -10,13 +13,17 @@ Variant LockState :=
 | LockIdle
 | LockAcqRunning (i : ThreadName)
 | LockOwned (i : ThreadName)
-| LockRelRunning (i : ThreadName).
+| LockRelRunning (i : ThreadName)
+| LockUB.
 
 Variant LockStep : LockState -> ThreadEvent LockSig -> LockState -> Prop :=
 | LockCallAcq i : LockStep LockIdle (i, CallEv Acq) (LockAcqRunning i)
 | LockRetAcq i : LockStep (LockAcqRunning i) (i, RetEv Acq tt) (LockOwned i)
 | LockCallRel i : LockStep (LockOwned i) (i, CallEv Rel) (LockRelRunning i)
-| LockRetRel i : LockStep (LockRelRunning i) (i, RetEv Rel tt) LockIdle.
+| LockRetRel i : LockStep (LockRelRunning i) (i, RetEv Rel tt) LockIdle
+| LockTwoAcq i : LockStep (LockAcqRunning i) (i, CallEv Acq) LockUB
+| LockTwoRel i : LockStep (LockRelRunning i) (i, CallEv Rel) LockUB
+| LockDoUB e : LockStep LockUB e LockUB.
 
 Definition lockSpec : Spec LockSig := {|
   State := LockState;
@@ -31,8 +38,23 @@ Definition OwnsLock i s :=
 
 Definition owner s :=
   match s with
-  | LockIdle => None
   | LockAcqRunning i => Some i
   | LockOwned i => Some i
   | LockRelRunning i => Some i
+  | _ => None
   end.
+
+Lemma owner_correct :
+  forall s i, owner s = Some i <-> OwnsLock i s.
+intros.
+split; intros.
+destruct s; simpl in *; try congruence.
+dependent destruction H. left. easy.
+dependent destruction H. right. left. easy.
+dependent destruction H. right. right. easy.
+destruct H.
+subst. easy.
+destruct H.
+subst. easy.
+subst. easy.
+Qed.
